Pollux.Proto.Prelude.fst
@@ -1,0 +1,18 @@
+module Pollux.Proto.Prelude 
+
+module U8 = FStar.UInt8
+
+type bytes = list U8.t
+
+(* The [option] monad *)
+// Bind operator
+let (let?) (x: option 'a) (f: 'a -> option 'b): option 'b
+  = match x with
+  | Some x -> f x
+  | None   -> None
+
+// Sort of applicative
+let (and?) (x: option 'a) (y: option 'b): option ('a & 'b)
+  = match x, y with
+  | Some x, Some y -> Some (x, y)
+  | _ -> None
